 \[
  \begin{array}{rcl}
    \selectedNonTerminal{E} &\Rightarrow& \nonterminal{E} * \selectedNonTerminal{E} \\
      &\Rightarrow& \nonterminal{E} * ( \selectedNonTerminal{E} )\\
      &\Rightarrow& \nonterminal{E} * ( \nonterminal{E} + \selectedNonTerminal{E} )\\
      &\Rightarrow& \nonterminal{E} * ( \selectedNonTerminal{E} + x )\\
      &\Rightarrow& \selectedNonTerminal{E} * ( z + x ) \\
      &\Rightarrow& (\selectedNonTerminal{E}) * ( z + x )\\
      &\Rightarrow& (\nonterminal{E} + \selectedNonTerminal{E} )*(z+x)\\
      &\Rightarrow& (\selectedNonTerminal{E}+y)*(z+x)\\
      &\Rightarrow& (x+y)*(z+x)\\
  \end{array}
  \]